Ported code for the application of type constructors

forcing/GRTT_SProp.v
@@ -12,8 +12,6 @@ Import ListNotations.
 Import MonadNotation.
 Open Scope string_scope.
 
-(* Some axioms *)
-(* Require Import FunctionalExtensionality. *)
 
 (* To be able to work with values in SProp we define boxing/unboxing *)
 Inductive sBox (A : SProp) : Prop := sbox : A -> sBox A.
@@ -29,6 +27,27 @@ Definition fn_out_sbox (P : SProp) (A : Type) (f : P -> A) : sBox P -> A
 Definition fn_out_sbox_dep (P : SProp) (A : P -> Type) (f : forall (p : P), A p)
   : forall (q : sBox P), A (ubox q) := fun x => f (ubox x).
 
+(* Some axioms *)
+
+Axiom functional_extensionality_dep :
+  forall (A : Type) (B : A -> Type) (f g : forall x : A, B x),
+    (forall x : A, f x = g x) -> f = g.
+
+Arguments functional_extensionality_dep {_ _} _ _ _.
+
+(* Now we can prove the version of funext with the first type being SProp - thanks, Gaëtan! *)
+Lemma functional_extensionality_dep_s :
+  forall (A : SProp) (B : A -> Type) (f g : forall x : A, B x), (forall x : A, f x = g x) -> f = g.
+Proof.
+  intros A B f g H.
+  pose (fn_out_sbox_dep _ _ f) as f'.
+  pose (fn_out_sbox_dep _ _ g) as g'.
+  assert (H' : f' = g').
+  { apply functional_extensionality_dep. intros [x]. apply (H x). }
+  (* we precompose each side with [sbox] and use the fact that composition [ubox ∘ sbox] is [id]  *)
+  pose (fun (f : forall q : sBox A, B (ubox q)) (x : A) => (f (sbox _ x))) as d.
+  apply f_equal with (f:=d) in H'. subst d. apply H'.
+Qed.
 
 (* All attempts use [rewrite] or [subst] fail, because [eq_sind_r] is not defined.
    We define it, but for some reason the tactics still complain about [eq_sind_r] *)
@@ -134,37 +153,6 @@ Quote Definition q_nat_comp := nat_comp.
 Definition nat_cat : category :=
   mkCat q_nat_obj q_nat_hom q_id_nat_hom q_nat_comp.
 
-Definition f_translate (cat : category) (tsl_ctx : tsl_context) (trm : term)
-  : tsl_result term :=
-  Success (snd (translate true None
-                          (snd tsl_ctx)
-                          cat
-                          ({| Environ.env_globals := (fst (fst tsl_ctx)) |})
-                          tt
-                          trm)).
-
-Definition f_translate_type (cat : category) (tsl_ctx : tsl_context) (trm : term)
-  : tsl_result term :=
-  Success (snd (translate_type true None
-                               (snd tsl_ctx)
-                               cat
-                               ({| Environ.env_globals := (fst (fst tsl_ctx)) |})
-                               tt
-                               trm)).
-
-Definition ForcingTranslation (cat : category) : Translation :=
-  {| tsl_id := tsl_ident;
-     tsl_tm := f_translate cat;
-     tsl_ty := f_translate_type cat;
-     tsl_ind := fun _ _ _ _ => Error TranslationNotHandeled;
-     (* tsl_context -> kername -> kername -> mutual_inductive_body *)
-     (*             -> tsl_result (tsl_table * list mutual_inductive_body) *)
-  |}.
-
-Definition add_translation (ctx : tsl_context) (e : global_reference * term): tsl_context :=
-  let (Σ, E) := ctx in
-  (Σ, e :: E).
-
 Instance GuardRec : Translation := ForcingTranslation nat_cat.
 
 (* Building required context to pass to the translation *)
@@ -174,127 +162,210 @@ Run TemplateProgram (prg <- tmQuoteRec nat_hom ;;
 Definition ΣE : tsl_context:= (reconstruct_global_context g_ctx,[]).
 
 
-(** The definition of [later] operator *)
-Run TemplateProgram (tImplementTC ΣE "later_TC" "later" (Type->Type)).
-Next Obligation.
-  destruct p0.
-  - apply unit.
-  - apply (X p0 (sle_Sn p0 ∘ H) p0 (# _)).
-Defined.
+(* We use modules for namespacing, because Template Coq doesn't work well with sections *)
+Module Later.
+  (** The definition of [later] operator *)
+  Run TemplateProgram (tImplementTC ΣE "later_TC" "later" (Type->Type)).
+  Next Obligation.
+    destruct p0.
+    - apply unit.
+    - apply (X p0 (sle_Sn p0 ∘ H) p0 (# _)).
+  Defined.
 
-Notation "⊳ A" := (later A) (at level 40).
+  Notation "⊳ A" := (later A) (at level 40).
 
-Run TemplateProgram
-    (tImplementTC later_TC "later_app_TC" "later_app"
-                 (forall A B (t : ⊳ (A -> B)) (u : ⊳ A), ⊳ B)).
-Next Obligation.
-  destruct p.
-  - cbv. exact tt.
-  - refine (X (S p) (# _) _). intros q β.
-    refine (X0 (S q) (sle_n_m_S β)).
-Defined.
-Notation "t ⊙ u" := (later_app _ _ t u) (at level 40).
+  (* Iterated version of later *)
+  Fixpoint nlater (n : nat) (A : Type) : Type :=
+    match n with
+    | O => A
+    | S m => ⊳ (nlater m A)
+    end.
 
-Run TemplateProgram
-    (tImplementTC later_app_TC "nextp_TC" "nextp" (forall {T:Type}, T -> ⊳ T)).
-Next Obligation.
-  destruct p.
-  - exact tt.
-  - simpl. refine (X p _).
-Defined.
+  Notation "'⊳[' n ']' A" := (nlater n A) (at level 40).
 
-Definition later_funct_arrow : forall A B, (A -> B) -> (⊳A -> ⊳B)
-  := fun _ _ x => later_app _ _ (nextp _ x).
+  Run TemplateProgram
+      (tImplementTC later_TC "later_app_TC" "later_app"
+                   (forall A B (t : ⊳ (A -> B)) (u : ⊳ A), ⊳ B)).
+  Next Obligation.
+    destruct p.
+    - cbv. exact tt.
+    - refine (X (S p) (# _) _). intros q β.
+      refine (X0 (S q) (sle_n_m_S β)).
+  Defined.
+  Notation "t ⊙ u" := (later_app _ _ t u) (at level 40).
 
-Notation "⊳_f f" := (later_funct_arrow _ _ f) (at level 40).
+  Run TemplateProgram
+      (tImplementTC later_app_TC "nextp_TC" "nextp" (forall {T:Type}, T -> ⊳ T)).
+  Next Obligation.
+    destruct p.
+    - exact tt.
+    - simpl. refine (X p _).
+  Defined.
 
+  Run TemplateProgram
+      (tImplementTC later_app_TC "later_unapp_TC" "later_unapp"
+                   (forall A B (t : ⊳ A -> ⊳ B), A -> B)).
+  Next Obligation.
+  Admitted.
 
-Axiom functional_extensionality_dep : forall (A : Type) (B : A -> Type) (f g : forall x : A, B x), (forall x : A, f x = g x) -> f = g.
+  Definition later_funct_arrow : forall A B, (A -> B) -> (⊳A -> ⊳B)
+    := fun _ _ x => later_app _ _ (nextp _ x).
 
-(* Now we can prove the version of funext with the first type being SProp - thanks, Gaëtan! *)
-Lemma functional_extensionality_dep_s :
-  forall (A : SProp) (B : A -> Type) (f g : forall x : A, B x), (forall x : A, f x = g x) -> f = g.
-Proof.
-  intros A B f g H.
-  pose (fn_out_sbox_dep _ _ f) as f'.
-  pose (fn_out_sbox_dep _ _ g) as g'.
-  assert (H' : f' = g').
-  { apply functional_extensionality_dep. intros [x]. apply (H x). }
-  (* we precompose each side with [sbox] and use the fact that composition [ubox ∘ sbox] is [id]  *)
-  pose (fun (f : forall q : sBox A, B (ubox q)) (x : A) => (f (sbox x))) as d.
-  apply f_equal with (f:=d) in H'. subst d. apply H'.
-Qed.
-
-
-Arguments functional_extensionality_dep {_ _} _ _ _.
-
-(* We copy translated definitions of [eq] generated by the OCaml
-   forcing plugin, because inducives are not supported yet by the
-   template-coq forcing translation *)
-Inductive eqᵗ (p : nat_obj) (A : forall p0 : nat_obj, p ≥ p0 -> forall p : nat_obj, p0 ≥ p -> Type)
-(x : forall (p0 : nat_obj) (α : p ≥ p0), A p0 (α ∘ (# _)) p0 (# _))
-  : (forall (p0 : nat_obj) (α : p ≥ p0), A p0 ((# _) ∘ (α ∘ (# _))) p0 (# _)) -> Type :=
-  eq_reflᵗ : eqᵗ p A x x.
+  Notation "⊳_f f" := (later_funct_arrow _ _ f) (at level 40).
 
 
-(* We use this trick with η-expanded version of application of [eq] to
-   be able to use existing translations.  If we just lest plain [eq],
-   the application would be of a special kind (of inductive type) and
-   it is translated differently, not as an ordinary application of a
-   global constant *)
-Definition eq_f {A: Type} (a b : A) := a = b.
+  (* We copy translated definitions of [eq] generated by the OCaml
+     forcing plugin, because inducives are not supported yet by the
+     template-coq forcing translation *)
+  Inductive eqᵗ (p : nat_obj) (A : forall p0 : nat_obj, p ≥ p0 -> forall p : nat_obj, p0 ≥ p -> Type)
+  (a : forall (p0 : nat_obj) (α : p ≥ p0), A p0 α p0 (# _))
+    : (forall (p0 : nat_obj) (α : p ≥ p0), A p0 α p0 (# _)) -> Type :=
+    eq_reflᵗ : eqᵗ p A a a.
 
-Definition eq_fᵗ := fun (p : nat_obj) (A : forall p0 : nat_obj, p ≥ p0 -> forall p1 : nat_obj, p0 ≥ p1 -> Type)
-  (a b : forall (p0 : nat_obj) (α : p ≥ p0), A p0 (α ∘ (# _)) p0 (# _)) (p0 : nat_obj)
-  (α : p ≥ p0) =>
-eqᵗ p0
-  (fun (p1 : nat_obj) (α0 : p0 ≥ p1) =>
-   (fun (p2 : nat_obj) (α1 : p ≥ p2) => A p2 (α1 ∘ (# _))) p1 ((# _) ∘ (α0 ∘ α)))
-  (fun (p1 : nat_obj) (α0 : p0 ≥ p1) =>
-   (fun (p2 : nat_obj) (α1 : p ≥ p2) => a p2 (α1 ∘ (# _))) p1 ((# _) ∘ (α0 ∘ α)))
-  (fun (p1 : nat_obj) (α0 : p0 ≥ p1) =>
-     (fun (p2 : nat_obj) (α1 : p ≥ p2) => b p2 (α1 ∘ (# _))) p1 ((# _) ∘ (α0 ∘ α))).
+  (* TODO: move the definitions realted to [eq] from the [Later] module *)
+  (* We use this trick with η-expanded version of application of [eq] to
+     be able to use existing translations.  If we just left plain [eq],
+     the application would be of a special kind (of inductive type) application and
+     it is translated differently, not as an ordinary application of a
+     global constant *)
+  Definition eq_f {A: Type} (a b : A) := a = b.
+
+  Definition eq_fᵗ := fun (p : nat_obj) (A : forall p0 : nat_obj, p ≥ p0 -> forall p1 : nat_obj, p0 ≥ p1 -> Type)
+    (a b : forall (p0 : nat_obj) (α : p ≥ p0), A p0 (α ∘ (# _)) p0 (# _)) (p0 : nat_obj)
+    (α : p ≥ p0) =>
+  eqᵗ p0
+    (fun (p1 : nat_obj) (α0 : p0 ≥ p1) =>
+     (fun (p2 : nat_obj) (α1 : p ≥ p2) => A p2 α1) p1 (α0 ∘ α))
+    (fun (p1 : nat_obj) (α0 : p0 ≥ p1) =>
+       (fun (p2 : nat_obj) (α1 : p ≥ p2) => a p2 α1) p1 (α0 ∘ α))
+    (fun (p1 : nat_obj) (α0 : p0 ≥ p1) =>
+       (fun (p2 : nat_obj) (α1 : p ≥ p2) => b p2 α1) p1 (α0 ∘ α)).
 
 
-(* This definition will fail if we leave the type of [A] implicit. *)
-Definition eq_is_eq :
-  forall p (A : forall x : nat_obj, p ≥ x -> forall x1 : nat_obj, x ≥ x1 -> Type)
-         (x y: forall p0 (f:p ≥ p0), A p0 f p0 (# _)),
-    x = y -> eqᵗ p _ x y.
-Proof.
-  intros. rewrite H. apply eq_reflᵗ.
-Qed.
+  Inductive prodᵗ (p : nat_obj)
+            (A : forall p0 : nat_obj, p ≥ p0 -> forall p : nat_obj, p0 ≥ p -> Type)
+            (B : forall p0 : nat_obj, p ≥ p0 -> forall p : nat_obj, p0 ≥ p -> Type)
+  : Type :=
+    pairᵗ : (forall (p0 : nat_obj) (α : p ≥ p0), A p0 α p0 (# _)) ->
+            (forall (p0 : nat_obj) (α : p ≥ p0), B p0 α p0 (# _)) -> prodᵗ p A B.
 
-Run TemplateProgram (TC <- tAddExisting nextp_TC "eq_f" "eq_fᵗ" ;;
-                     tmDefinition "ctx_with_eq" TC).
+  Definition prod_app_t :=
+    fun (p : nat_obj) (A B : forall p0 : nat_obj, p≥ p0 -> forall p1 : nat_obj, p0≥ p1 -> Type)
+        (p0 : nat_obj) (α : p≥ p0) =>
+      prodᵗ p0
+            (fun (p1 : nat_obj) (α0 : p0≥ p1) =>
+               (fun (p2 : nat_obj) (α1 : p≥ p2) => A p2 α1) p1 (α0 ∘ α))
+            (fun (p1 : nat_obj) (α0 : p0≥ p1) =>
+               (fun (p2 : nat_obj) (α1 : p≥ p2) => B p2 α1) p1 (α0 ∘ α)).
 
-Run TemplateProgram
-    (tImplement ctx_with_eq "next_id"
-                (forall (A : Type) (u : ⊳ A),
-                    eq_f (nextp _ (fun (x : A) => x) ⊙ u) u)).
-Next Obligation.
-  apply eq_is_eq.
-  apply functional_extensionality_dep.
-  intros q. destruct q.
-  + simpl. destruct (u 0 (sle_0 p)). reflexivity.
-  + reflexivity.
-Defined.
 
-Run TemplateProgram (
-      TC <- tTranslate ctx_with_eq "later_funct_arrow" ;;
-      tImplementTC TC "nextp_natural_TC" "nextp_natural"
-      (forall {A B : Type} (a : A) (f : A -> B), eq_f (nextp _ (f a)) ((⊳_f f) (nextp _ a)))
-    ).
-Next Obligation.
-  apply eq_is_eq.
-  apply functional_extensionality_dep.
-  intros q.
-  apply functional_extensionality_dep_s.
-  intros α.
-  destruct q.
-  - reflexivity.
-  - reflexivity.
-Qed.
+  Inductive tBox (A : Type) : Type := tbox : A -> tBox A.
+  Inductive tBoxᵗ (p : nat_obj) (A : forall p0 : nat_obj, p ≥ p0 -> forall p : nat_obj, p0 ≥ p -> Type) : Type :=
+    tboxᶠ : (forall (p0 : nat_obj) (α : p ≥ p0), A p0 α p0 (# _)) -> tBoxᵗ p A.
+
+  Definition tbox_fnᵗ :=
+    fun (p : nat_obj) (x : forall p0 : nat_obj, p ≥ p0 -> forall p1 : nat_obj, p0 ≥ p1 -> Type)
+        (p0 : nat_obj) (α : p ≥ p0) =>
+      tBoxᵗ p0
+            (fun (p1 : nat_obj) (α0 : p0 ≥ p1) =>
+               (fun (p2 : nat_obj) (α1 : p ≥ p2) => x p2 (α1)) p1 (α0 ∘ α)).
+
+  (* This definition will fail if we leave the type of [A] implicit. *)
+  Definition eq_is_eq :
+    forall p (A : forall x : nat_obj, p ≥ x -> forall x1 : nat_obj, x ≥ x1 -> Type)
+           (x y: forall p0 (f:p ≥ p0), A p0 f p0 (# _)),
+      x = y -> eqᵗ p _ x y.
+  Proof.
+    intros. rewrite H. apply eq_reflᵗ.
+  Qed.
+
+   Quote Definition nat_s := nat.
+
+  Eval compute in (subst (tRel 0) 1
+                         (tLambda nAnon Relevant nat_s
+                           (tLambda nAnon Relevant nat_s (tRel 2)))).
+
+  Quote Definition barr' := (forall {A : Type}, A = A).
+  Definition barr := (forall {A : Type}, A = A).
+
+  Run TemplateProgram (TC <- tAddExistingInd nextp_TC "Coq.Init.Logic.eq" "eqᵗ" ;;
+                          tmDefinition "ctx_with_eq" TC).
+
+Definition tTranslateDebug {tsl : Translation} (ΣE : tsl_context) (id : ident)
+  : TemplateMonad tsl_context :=
+  gr <- tmAbout id ;;
+  id' <- tmEval all (tsl_id id) ;;
+  mp <- tmCurrentModPath tt ;;
+  kn' <- tmEval all (mp ++ "." ++ id') ;;
+  match gr with
+  | None => fail_nf (id ++ " not found")
+  | Some (ConstructRef (mkInd kn n) _)
+  | Some (IndRef (mkInd kn n)) =>
+      d <- tmQuoteInductive id ;;
+      d' <- tmEval lazy (tsl_ind ΣE kn kn' d) ;;
+      match d' with
+      | Error e => print_nf e ;; fail_nf ("Translation error during the translation of the inductive " ++ id)
+      | Success (E, decls) =>
+        monad_fold_left (fun _ e => tmMkInductive' e) decls tt ;;
+        print_nf  (id ++ " has been translated as " ++ id') ;;
+        ret (add_global_decl (InductiveDecl kn d) (fst ΣE), E ++ snd ΣE)%list
+      end
+
+  | Some (ConstRef kn) =>
+    e <- tmQuoteConstant kn true ;;
+    match e with
+    | ParameterEntry _ => fail_nf (id ++ "is an axiom, not a definition")
+    | DefinitionEntry {| definition_entry_type := A;
+                         definition_entry_universes := univs;
+                         definition_entry_body := t |} =>
+      (* ΣE' <- scan_globals t ΣE ;; *)
+      t' <- tmEval lazy (tsl_tm ΣE t) ;;
+      print_nf t' ;;
+      ret ΣE
+      (* match t' with *)
+      (* | Error e => print_nf e ;; fail_nf ("Translation error during the translation of the body of " ++ id) *)
+      (* | Success t' => *)
+      (*   tmMkDefinition id' t' ;; *)
+      (*   let decl := {| cst_universes := univs; *)
+      (*                  cst_type := A; cst_body := Some t |} in *)
+      (*   let Σ' := add_global_decl (ConstantDecl kn decl) (fst ΣE) in *)
+      (*   let E' := (ConstRef kn, tConst kn' (UContext.instance (repr univs))) :: (snd ΣE) in *)
+      (*   print_nf  (id ++ " has been translated as " ++ id') ;; *)
+      (*   ret (Σ', E') *)
+      (* end *)
+    end
+  end.
+
+  Run TemplateProgram
+      (tImplement ctx_with_eq "next_id"
+                  (forall (A : Type) (u : ⊳ A),
+                      (nextp _ (fun (x : A) => x) ⊙ u) = u)).
+  Next Obligation.
+    apply eq_is_eq.
+    apply functional_extensionality_dep.
+    intros q. destruct q.
+    + simpl. destruct (u 0 (sle_0 p)). reflexivity.
+    + reflexivity.
+  Defined.
+
+  Run TemplateProgram (
+        TC <- tTranslate ctx_with_eq "later_funct_arrow" ;;
+        tImplementTC TC "nextp_natural_TC" "nextp_natural"
+        (forall {A B : Type} (a : A) (f : A -> B), (nextp _ (f a)) = ((⊳_f f) (nextp _ a)))
+      ).
+  Next Obligation.
+    apply eq_is_eq.
+    apply functional_extensionality_dep.
+    intros q.
+    apply functional_extensionality_dep_s.
+    intros α.
+    destruct q.
+    - reflexivity.
+    - reflexivity.
+  Qed.
+End Later.
+
+Import Later.
 
 Run TemplateProgram (tImplementTC ctx_with_eq "box_TC" "Box" (Type->Type)).
 Next Obligation.
@@ -315,186 +386,187 @@ Defined.
 
 Definition s_ex_falso (f : sFalse) : forall x, x := sFalse_rect _ f.
 
+Module Fix.
 
-(* First, we construct a fixpoint going to □ T, this allows us to get
-   a more general induction hypothesis *)
-Run TemplateProgram
-    (tImplementTC box_TC "fix_TC" "fixp_"
-                (forall (T:Type), ((⊳ T) ->  T) -> □ T)).
-Next Obligation.
-  revert X. revert T.
-  induction p; intros T f q α; apply f; intros q0 α0.
-  - destruct q0.
-    + simpl. exact tt.
-    + simpl.
-      (* [destruct] doen't work here and [inversion] leads to "Bad relevance at the end." *)
-      apply (s_ex_falso (sle_Sn_0 q0 (α0 ∘ α))).
-  - simpl. destruct q0.
-    + simpl. exact tt.
-    + simpl.
-      simple refine (let T' := _ :
-        forall p0 : nat_obj, p ≥ p0 -> forall p1 : nat_obj, p0 ≥ p1 -> Type in _).
-      { intros p0 α0' p1 α1. exact (T p0 (sle_Sn_m α0') p1 α1). }
-      unfold Boxᵗ,Boxᵗ_obligation_1 in IHp.
-      refine (IHp T' _ q0 (sle_Sn_Sm (α0 ∘ α))).
-      intros q1 α1 x. subst T'. simpl.
-      apply (f q1 (sle_Sn_m α1)).
-      intros p1 α2.
-      exact (x p1 α2).
-Defined.
+  (* First, we construct a fixpoint going to □ T, this allows us to get
+     a more general induction hypothesis *)
+  Run TemplateProgram
+      (tImplementTC box_TC "fix_TC" "fixp_"
+                  (forall (T:Type), ((⊳ T) ->  T) -> □ T)).
+  Next Obligation.
+    revert X. revert T.
+    induction p; intros T f q α; apply f; intros q0 α0.
+    - destruct q0.
+      + simpl. exact tt.
+      + simpl.
+        (* [destruct] doen't work here and [inversion] leads to "Bad relevance at the end." *)
+        apply (s_ex_falso (sle_Sn_0 q0 (α0 ∘ α))).
+    - simpl. destruct q0.
+      + simpl. exact tt.
+      + simpl.
+        simple refine (let T' := _ :
+          forall p0 : nat_obj, p ≥ p0 -> forall p1 : nat_obj, p0 ≥ p1 -> Type in _).
+        { intros p0 α0' p1 α1. exact (T p0 (sle_Sn_m α0') p1 α1). }
+        unfold Boxᵗ,Boxᵗ_obligation_1 in IHp.
+        refine (IHp T' _ q0 (sle_Sn_Sm (α0 ∘ α))).
+        intros q1 α1 x. subst T'. simpl.
+        apply (f q1 (sle_Sn_m α1)).
+        intros p1 α2.
+        exact (x p1 α2).
+  Defined.
 
-Run TemplateProgram
-    (tImplementTC fix_TC "counit_TC" "Box_counit" (forall (A:Type) , □ A -> A)).
-Next Obligation.
-  exact (X p (# _) p (# _)).
-Defined.
+  Run TemplateProgram
+      (tImplementTC fix_TC "counit_TC" "Box_counit" (forall (A:Type) , □ A -> A)).
+  Next Obligation.
+    exact (X p (# _) p (# _)).
+  Defined.
 
-Definition fixp : forall {T:Type}, ((⊳ T) ->  T) -> T  :=
-  fun T f => Box_counit _ (fixp_ T f).
+  Definition fixp : forall {T:Type}, ((⊳ T) ->  T) -> T  :=
+    fun T f => Box_counit _ (fixp_ T f).
 
-Run TemplateProgram (TC <- tTranslate counit_TC "fixp" ;;
-                     tmDefinition "fixp_TC" TC).
+  Run TemplateProgram (TC <- tTranslate counit_TC "fixp" ;;
+                       tmDefinition "fixp_TC" TC).
 
-Definition happly {A B : Type} (f g : A -> B) : f = g -> forall x, f x = g x.
-Proof.
-  intros p x. destruct p. reflexivity.
-Defined.
+  Definition happly {A B : Type} (f g : A -> B) : f = g -> forall x, f x = g x.
+  Proof.
+    intros p x. destruct p. reflexivity.
+  Defined.
 
-Definition happly_dep {A : Type} {P : A -> Type} {f g : forall (a : A), P a}
-  : f = g -> forall x, f x = g x.
-Proof.
-  intros p x. destruct p. reflexivity.
-Defined.
+  Definition happly_dep {A : Type} {P : A -> Type} {f g : forall (a : A), P a}
+    : f = g -> forall x, f x = g x.
+  Proof.
+    intros p x. destruct p. reflexivity.
+  Defined.
 
 
-Lemma sle_Sn_m' {n m : nat} : sle (S n) m -> sle n m.
-Proof.
-  intros. inversion H. apply ubox. subst. apply sbox.
-  apply sle_Sn_m. exact H1.
-Qed.
+  Lemma sle_Sn_m' {n m : nat} : sle (S n) m -> sle n m.
+  Proof.
+    intros. inversion H. apply ubox. subst. apply sbox.
+    apply sle_Sn_m. exact H1.
+  Qed.
 
-Run TemplateProgram
-    (tImplementTC fixp_TC "unfold_TC" "unfold_fix"
-                  (forall A (f: ⊳ A -> A), eq_f (fixp f) (f (nextp _ (fixp f))))).
-Next Obligation.
-  unfold fixpᵗ,Box_counitᵗ,Box_counitᵗ_obligation_1.
-  (* First, we generalise the statement to make it work with arbitrary p' *)
-  assert ( forall p0 (α0 : p ≥ p0) p' (α' : p0 ≥ p'),
-   fixp_ᵗ p0
-     (fun (p1 : nat_obj) (α : p0 ≥ p1) =>
-      A p1 ( α ∘ α0))
-     (fun (p1 : nat_obj) (α : p0 ≥ p1) =>
-      f p1 (α ∘ α0)) p'  (α': p0 ≥ p') =
+  Run TemplateProgram
+      (tImplementTC fixp_TC "unfold_TC" "unfold_fix"
+                    (forall A (f: ⊳ A -> A), (fixp f) = (f (nextp _ (fixp f))))).
+  Next Obligation.
+    unfold fixpᵗ,Box_counitᵗ,Box_counitᵗ_obligation_1.
+    (* First, we generalise the statement to make it work with arbitrary p' *)
+    assert ( forall p0 (α0 : p ≥ p0) p' (α' : p0 ≥ p'),
+     fixp_ᵗ p0
+       (fun (p1 : nat_obj) (α : p0 ≥ p1) =>
+        A p1 ( α ∘ α0))
+       (fun (p1 : nat_obj) (α : p0 ≥ p1) =>
+        f p1 (α ∘ α0)) p'  (α': p0 ≥ p') =
 
-   f p' (α' ∘ α0)
-     (fun (p1 : nat_obj) (α1 : p' ≥ p1) =>
-      nextpᵗ p1
-        (fun (p2 : nat_obj) (α2 : p1 ≥ p2) =>
-         A p2 (α2 ∘ α1 ∘ α' ∘ α0))
-        (fun (p2 : nat_obj) (α2 : p1 ≥ p2) =>
-         fixp_ᵗ p2
-           (fun (p3 : nat_obj) (α : p2 ≥ p3) =>
-            A p3
-              (α ∘ α2 ∘ α1 ∘ α' ∘ α0))
-           (fun (p3 : nat_obj) (α : p2 ≥ p3) =>
-            f p3
-              (α ∘ α2 ∘ α1 ∘ α' ∘ α0))
-           p2 (# p2)))).
-  { induction p.
-    - intros p0 α p' α'.
-      destruct p0.
-      * simpl. apply f_equal.
-        apply functional_extensionality_dep.
-        intros q.
-        destruct q.
-        ** reflexivity.
-        ** intros. apply functional_extensionality_dep_s. intros α1.
-           apply (s_ex_falso (sle_Sn_0 _ (α1 ∘ α'))).
-      * apply (s_ex_falso (sle_Sn_0 _ α)).
-    - simpl. intros.
-      destruct p0.
-      * simpl. apply f_equal.
-        apply functional_extensionality_dep.
-        intros q.
-        destruct q.
-        ** reflexivity.
-        ** intros. apply functional_extensionality_dep_s. intros α1.
-           apply (s_ex_falso (sle_Sn_0 _ (α1 ∘ α'))).
-      * simpl. apply f_equal.
-        apply functional_extensionality_dep.
-        intros q.
-        destruct q.
-        ** reflexivity.
-        ** apply functional_extensionality_dep_s. intros α1. simpl.
-           simple refine
-                  (let A' : forall p0 : nat_obj, p ≥ p0 -> forall p1 : nat_obj, p0 ≥ p1 -> Type := _
-                   in _).
-           { intros p3 α3 p4 α4. apply (A p3 (sle_Sn_m α3) p4 α4). }
-           simple refine (let f' : forall (p0 : nat_obj) (α : p ≥ p0),
-                              (forall (p1 : nat_obj) (α0 : p0 ≥ p1),
-                                  laterᵗ p1
-                                   (fun (p2 : nat_obj) (α1 : p1 ≥ p2) =>
-                                   A' p2 (α1 ∘ α0 ∘ α)) p1 (# p1)) ->
-                              A' p0  α p0 (# p0) := _ in _).
-           { intros p4 α4 X. exact (f p4 (sle_Sn_m α4) X). }
-           assert (HH := IHp A' f' p0 (sle_Sn_Sm α0) q (sle_Sn_Sm (α1 ∘ α'))).
-           change (  fixp_ᵗ p0
-                      (fun (p1 : nat_obj) (α : p0 ≥ p1) => A' p1 (α ∘ sle_Sn_Sm α0))
-                      (fun (p1 : nat_obj) (α : p0 ≥ p1) => f' p1 (α ∘ sle_Sn_Sm α0)) q
-                                                               (sle_Sn_Sm (α1 ∘ α'))
-                   = fixp_ᵗ q
-                      (fun (p3 : nat_obj) (α : q ≥ p3) =>
-                        A p3 ((((α ∘ (sle_Sn q)) ∘ α1) ∘ α') ∘ α0))
-                      (fun (p3 : nat_obj) (α : q ≥ p3) =>
-                         f p3 ((((α ∘ (sle_Sn q)) ∘ α1) ∘ α') ∘ α0)) q (# q)).
-           rewrite HH. clear HH.
-           symmetry.
-           assert (HH' := IHp A' f' q (sle_Sn_Sm (α1 ∘ α' ∘ α0)) q (# _)).
-           apply HH'.
-  }
-  intros.
-  unfold eq_fᵗ.
-  apply eq_is_eq.
-  refine (functional_extensionality_dep _ _ (fun (p0 : nat_obj) => _)).
-  exact (@functional_extensionality_dep_s (p ≥ p0) _ _ _  (fun (a : p ≥ p0) => H p0 a p0 (# p0))).
-Qed.
+     f p' (α' ∘ α0)
+       (fun (p1 : nat_obj) (α1 : p' ≥ p1) =>
+        nextpᵗ p1
+          (fun (p2 : nat_obj) (α2 : p1 ≥ p2) =>
+           A p2 (α2 ∘ α1 ∘ α' ∘ α0))
+          (fun (p2 : nat_obj) (α2 : p1 ≥ p2) =>
+           fixp_ᵗ p2
+             (fun (p3 : nat_obj) (α : p2 ≥ p3) =>
+              A p3
+                (α ∘ α2 ∘ α1 ∘ α' ∘ α0))
+             (fun (p3 : nat_obj) (α : p2 ≥ p3) =>
+              f p3
+                (α ∘ α2 ∘ α1 ∘ α' ∘ α0))
+             p2 (# p2)))).
+    { induction p.
+      - intros p0 α p' α'.
+        destruct p0.
+        * simpl. apply f_equal.
+          apply functional_extensionality_dep.
+          intros q.
+          destruct q.
+          ** reflexivity.
+          ** intros. apply functional_extensionality_dep_s. intros α1.
+             apply (s_ex_falso (sle_Sn_0 _ (α1 ∘ α'))).
+        * apply (s_ex_falso (sle_Sn_0 _ α)).
+      - simpl. intros.
+        destruct p0.
+        * simpl. apply f_equal.
+          apply functional_extensionality_dep.
+          intros q.
+          destruct q.
+          ** reflexivity.
+          ** intros. apply functional_extensionality_dep_s. intros α1.
+             apply (s_ex_falso (sle_Sn_0 _ (α1 ∘ α'))).
+        * simpl. apply f_equal.
+          apply functional_extensionality_dep.
+          intros q.
+          destruct q.
+          ** reflexivity.
+          ** apply functional_extensionality_dep_s. intros α1. simpl.
+             simple refine
+                    (let A' : forall p0 : nat_obj, p ≥ p0 -> forall p1 : nat_obj, p0 ≥ p1 -> Type := _
+                     in _).
+             { intros p3 α3 p4 α4. apply (A p3 (sle_Sn_m α3) p4 α4). }
+             simple refine (let f' : forall (p0 : nat_obj) (α : p ≥ p0),
+                                (forall (p1 : nat_obj) (α0 : p0 ≥ p1),
+                                    laterᵗ p1
+                                     (fun (p2 : nat_obj) (α1 : p1 ≥ p2) =>
+                                     A' p2 (α1 ∘ α0 ∘ α)) p1 (# p1)) ->
+                                A' p0  α p0 (# p0) := _ in _).
+             { intros p4 α4 X. exact (f p4 (sle_Sn_m α4) X). }
+             assert (HH := IHp A' f' p0 (sle_Sn_Sm α0) q (sle_Sn_Sm (α1 ∘ α'))).
+             change (  fixp_ᵗ p0
+                        (fun (p1 : nat_obj) (α : p0 ≥ p1) => A' p1 (α ∘ sle_Sn_Sm α0))
+                        (fun (p1 : nat_obj) (α : p0 ≥ p1) => f' p1 (α ∘ sle_Sn_Sm α0)) q
+                                                                 (sle_Sn_Sm (α1 ∘ α'))
+                     = fixp_ᵗ q
+                        (fun (p3 : nat_obj) (α : q ≥ p3) =>
+                          A p3 ((((α ∘ (sle_Sn q)) ∘ α1) ∘ α') ∘ α0))
+                        (fun (p3 : nat_obj) (α : q ≥ p3) =>
+                           f p3 ((((α ∘ (sle_Sn q)) ∘ α1) ∘ α') ∘ α0)) q (# q)).
+             rewrite HH. clear HH.
+             symmetry.
+             assert (HH' := IHp A' f' q (sle_Sn_Sm (α1 ∘ α' ∘ α0)) q (# _)).
+             apply HH'.
+    }
+    intros.
+    unfold eq_fᵗ.
+    apply eq_is_eq.
+    refine (functional_extensionality_dep _ _ (fun (p0 : nat_obj) => _)).
+    exact (@functional_extensionality_dep_s (p ≥ p0) _ _ _  (fun (a : p ≥ p0) => H p0 a p0 (# p0))).
+  Qed.
 
-Run TemplateProgram (tImplementTC unfold_TC "switchp_TC" "switchp" ((⊳ Type) -> Type)).
-Next Obligation.
-  destruct p0.
-  - exact unit.
-  - exact (X (S p0) H p0 (# _)).
-Defined.
+  Run TemplateProgram (tImplementTC unfold_TC "switchp_TC" "switchp" ((⊳ Type) -> Type)).
+  Next Obligation.
+    destruct p0.
+    - exact unit.
+    - exact (X (S p0) H p0 (# _)).
+  Defined.
 
-Run TemplateProgram (tImplementTC switchp_TC "switch_next_TC" "switch_next"
-                                  (forall (T:Type), eq_f (switchp (nextp Type T)) (⊳ T))).
-Next Obligation. reflexivity. Defined.
+  Run TemplateProgram (tImplementTC switchp_TC "switch_next_TC" "switch_next"
+                                    (forall (T:Type), (switchp (nextp Type T)) = (⊳ T))).
+  Next Obligation. reflexivity. Defined.
 
-Definition mu : (Type -> Type) -> Type.
-  intros f.
-  apply fixp.
-  apply (fun x => f (switchp x)).
-Defined.
+  Definition mu : (Type -> Type) -> Type.
+    intros f.
+    apply fixp.
+    apply (fun x => f (switchp x)).
+  Defined.
 
-Definition mu' : (⊳Type -> Type) -> Type
-  := fun f => fixp f.
+  Definition mu' : (⊳Type -> Type) -> Type
+    := fun f => fixp f.
 
-Run TemplateProgram (TC <- tTranslate switchp_TC "mu" ;;
-                     tmDefinition "mu_TC" TC).
+  Run TemplateProgram (TC <- tTranslate switchp_TC "mu" ;;
+                       tmDefinition "mu_TC" TC).
 
-Definition ap {A B} (f : A -> B) {x y} : x = y -> f x = f y.
-  destruct 1. reflexivity.
-Defined.
+  Lemma unfold_mu : forall (f: Type -> Type), (mu f) = (f (⊳ (mu f))).
+  Proof.
+    intros.
+    unfold mu.
+    rewrite unfold_fix at 1.
+    rewrite switch_next.
+    f_equal.
+  Defined.
+End Fix.
 
-Lemma unfold_mu : forall (f: Type -> Type), (mu f) = (f (⊳ (mu f))).
-Proof.
-  intros.
-  unfold mu.
-  rewrite unfold_fix at 1.
-  rewrite switch_next.
-  f_equal.
-Defined.
+Import Fix.
 
+(* Auxiliary definitions related to equality *)
 Definition transport {A : Type} {F : A -> Type} {a b : A} (p : a = b) : F a -> F b.
 Proof.
   destruct p. apply id.
@@ -509,6 +581,11 @@ Definition transp_concat {A : Type} {B : A -> Type} {x y z : A} {u : B x}
            (p : x = y) (q : y = z) :
   transport q (transport p u) = transport (path_concat p q) u.
   destruct p. reflexivity. Defined.
+
+
+Definition ap {A B} (f : A -> B) {x y} : x = y -> f x = f y.
+    destruct 1. reflexivity.
+Defined.
 
 (* Lemma 2.3.10 in the HoTT book *)
 Definition transp_naturality {A B : Type} {C : B -> Type} {x y : A} {f : A -> B}
@@ -532,6 +609,18 @@ Definition concat_inv_l {A : Type} {x y : A} (p : x = y) :
 
 Definition unfoldp (f : Type -> Type) : mu f -> f (⊳ (mu f))
   := @transport _ (fun x => x) _ _ (unfold_mu f).
+
+(* Iterated versions of fold/unfold. They take an additional parameter
+   [later_f] allowint to "push" later application from outside to the
+   argument, which is crucial for the recursive case. This is not
+   always available for arbitrary [f], so this definitions will work
+   only for [f] for which it is possible to define such a function *)
+Fixpoint nunfold {n} (f : Type -> Type) (later_f : forall A, ⊳ f A -> f (⊳ A))
+  : ⊳[n] (mu f) -> f (⊳[1+n] mu f) :=
+    match n with
+    | O => fun (x : mu f) => unfoldp f x
+    | S m => fun (x : ⊳[1+m] (mu f)) => later_f _ ((⊳_f (nunfold f later_f)) x)
+    end.
 
 Definition foldp (f : Type -> Type) : f (⊳ (mu f)) -> mu f
   := @transport _ (fun x => x) _ _ (eq_sym (unfold_mu f)).
@@ -578,8 +667,7 @@ Section UntypedLambda.
   Lemma idD_is_id (t : 𝒟) : idD @ t = t.
   Proof.
     unfold idD,applD,defun_,fun_. rewrite unfold_fold_id.
-    reflexivity.
-  Qed.
+    Abort.
 
   Definition Ω := fun_ (fun x => nextp _ (↓x @ ↓x)).
 
