forcing/Tests.v
@@ -1,11 +1,12 @@
 (* Some sanity tests for several definitions. We test agaist the tranlation acquired from the OCaml
  forcing translation plugin (up to notation) *)
 Require Import Template.monad_utils Template.Ast
-        Template.Template Template.LiftSubst.
+        Template.Template Template.LiftSubst translation_utils.
 Require Import String PeanoNat.
 Require Import Forcing.TemplateForcing.
 
 Import List.ListNotations.
+Import MonadNotation.
 Open Scope string_scope.
 Open Scope list_scope.
 
@@ -38,7 +39,7 @@ Definition tr_Id_syn :=
                    {| Environ.env_globals := g_ctx|}
                    tt qId.
 
-(*A translation of [fun (x : Type) => x] from the original plugin *)
+(*A translation of [fun (x : Type) => x] from the OCaml plugin *)
 Definition fooᶠ  : forall p : Obj,
     (forall p0 : Obj, p ≥ p0 -> forall p1 : Obj, p0 ≥ p1 -> Type) ->
     forall p0 : Obj, p ≥ p0 -> Type
@@ -60,7 +61,7 @@ Definition tr_Arr_syn :=
                    tt qArr.
 
 
-(* Translation of [(fun (A B : Type)  => A -> B)] from the original plugin*)
+(* Translation of [(fun (A B : Type)  => A -> B)] from the OCaml plugin*)
 Definition barᶠ : forall p : Obj,
     (forall p0 : Obj, p ≥ p0 -> forall p1 : Obj, p0 ≥ p1 -> Type) ->
     (forall p0 : Obj, p ≥ p0 -> forall p1 : Obj, p0 ≥ p1 -> Type) ->
@@ -87,3 +88,37 @@ Definition tr_bazz_syn :=
 (* Just testing that the definition can be reflected back from quoted. This covers a bug with
    top-level condition variable when building a chain of moprhisms by composition *)
 Make Definition bazz' := Eval vm_compute in (snd tr_bazz_syn).
+
+
+(* Testing appication of type constructors *)
+
+Inductive prodᵗ (p : Obj)
+            (A : forall p0 : Obj, p ≥ p0 -> forall p : Obj, p0 ≥ p -> Type)
+            (B : forall p0 : Obj, p ≥ p0 -> forall p : Obj, p0 ≥ p -> Type)
+  : Type :=
+    pairᵗ : (forall (p0 : Obj) (α : p ≥ p0), A p0 α p0 (# _)) ->
+            (forall (p0 : Obj) (α : p ≥ p0), B p0 α p0 (# _)) -> prodᵗ p A B.
+
+(* translation of [fun (A B : Type) => prod A B] from the OCaml plugin *)
+Definition prod_app_t :=
+    fun (p : Obj) (A B : forall p0 : Obj, p≥ p0 -> forall p1 : Obj, p0≥ p1 -> Type)
+        (p0 : Obj) (α : p≥ p0) =>
+      prodᵗ p0
+            (fun (p1 : Obj) (α0 : p0≥ p1) =>
+               (fun (p2 : Obj) (α1 : p≥ p2) => A p2 α1) p1 (α0 ∘ α))
+            (fun (p1 : Obj) (α0 : p0≥ p1) =>
+               (fun (p2 : Obj) (α1 : p≥ p2) => B p2 α1) p1 (α0 ∘ α)).
+
+Instance TestTranslation : Translation := ForcingTranslation test_cat.
+
+Definition ΣE : tsl_context:= (Typing.reconstruct_global_context [],[]).
+
+Run TemplateProgram (TC <- tAddExistingInd ΣE "Coq.Init.Datatypes.prod" "prodᵗ" ;;
+                          tmDefinition "ctx_with_prod" TC).
+
+Definition prod_ := (fun (A B : Type) => prod A B).
+
+Run TemplateProgram (tTranslate ctx_with_prod "prod_").
+
+Lemma prod_tr_eq : prod_ᵗ = prod_app_t.
+Proof. reflexivity. Qed.
